DY/Actions/Random.lean
@@ -1,0 +1,243 @@
+module
+
+public import DY.Trace
+public import DY.Bytes
+public import DY.Trace.Manipulation
+public import DY.Misc.Instances
+import DY.Step.Init
+
+namespace DY.Random
+
+section Trace
+
+public
+structure ExecEntryT where
+  length: Nat
+
+public
+def attKnows [BytesFunctor] [ExecTraceTypes]: ExecEntryAttackerKnowledge ExecEntryT where
+  attackerKnows _ _ _ := False
+
+public
+structure ProofEntryT [BytesFunctor] [ExecTraceTypes] where
+  length: Nat
+  label: Label
+  usage: Usage
+
+public
+def ProofEntryFunc [BytesFunctor] [ExecTraceTypes]: ProofEntryFun ExecEntryT ProofEntryT where
+  erase | {length, label := _, usage := _} => { length }
+
+public
+def Invariant [BytesFunctor] [TraceTypes]: TraceEntryInvariant ProofEntryFunc where
+  invariant _ _ := True
+
+-- TODO attacker knowledge theorem
+
+end Trace
+
+section Bytes
+
+section Constructors
+
+public
+structure Random (Bytes: Type) where
+  timestamp: Nat
+  size: Nat
+
+public
+instance: ALaCarte.FunctorSizeOf Random where
+  sizeOf | {timestamp := _, size := _} => 0
+
+public
+instance: ALaCarte.Representable Random where
+  CtorId := Unit
+  ctors | () => { Data := Nat × Nat, nRec := 0 }
+
+  toRepr | {timestamp, size} => {
+    id := ()
+    data := (timestamp, size)
+    as := #v[]
+  }
+  fromRepr
+  | {id, data := (timestamp, size), as} =>
+    { timestamp, size }
+  from_to | {timestamp, size} => by rfl
+  to_from
+  | {id, data, as} => by
+    simp_all <;> grind
+  sizeOf_eq | {timestamp := _, size := _} => by simp +arith [ALaCarte.FunctorSizeOf.sizeOf]
+
+public instance: ALaCarte.RepresentableDecidableEq Random where
+public instance: ALaCarte.RepresentableOrd Random where
+  ctorDataOrd | () => Ord.lex inferInstance inferInstance
+
+public instance: SubBytesFunctor Random where
+
+public
+abbrev SubF := Random
+
+public
+def Random.length [BytesFunctor]: Bytes.PartialLength Random :=
+  fun { timestamp := _, size := size } _ =>
+    size
+
+public
+abbrev SubF.length [BytesFunctor]: Bytes.PartialLength SubF := Random.length
+
+public
+abbrev Random.pack [BytesFunctor] [BytesFunctor.Has SubF] (x: Random Bytes) := BytesView.pack x
+
+def makeRand [BytesFunctor] [BytesFunctor.Has SubF] (timestamp size: Nat): Bytes :=
+  ({timestamp, size}: Random Bytes).pack
+
+end Constructors
+
+section AttackerKnowledge
+
+variable [BytesFunctor] [BytesFunctor.Has SubF]
+
+public
+def attKnowsRand: SubAttackerKnowledge Random where
+  pred p out := False
+
+public
+abbrev attackerKnowledge := attKnowsRand
+
+end AttackerKnowledge
+
+section Invariants
+
+variable [TraceTypes]
+variable [BytesFunctor] [BytesFunctor.Has SubF]
+variable [TraceTypes.Has ProofEntryFunc]
+
+public
+def Random.invariants: Bytes.PartialInvariants Random where
+  well_formed := fun {timestamp, size} _rec tr =>
+    ∃ (label: Label) (usage: Usage),
+    tr.at_is timestamp ({length := size, label, usage}: ProofEntryT)
+
+  usage := fun {timestamp, size := _} _rec tr =>
+    if h_timestamp: timestamp < tr.length then
+      match TraceTypes.Has.proofProj (tr.at timestamp h_timestamp) with
+      | some (entry: ProofEntryT) =>
+        entry.usage
+      | none => Usage.nothing
+    else
+      Usage.nothing
+
+  label := fun {timestamp, size := _} _rec tr =>
+    if h_timestamp: timestamp < tr.length then
+      match TraceTypes.Has.proofProj (tr.at timestamp h_timestamp) with
+      | some (entry: ProofEntryT) =>
+        entry.label
+      | none => Label.pub
+    else
+      Label.pub
+
+  invariant := fun {timestamp, size} _rec tr =>
+    ∃ (label: Label) (usage: Usage),
+    tr.at_is timestamp ({length := size, label, usage}: ProofEntryT)
+
+public
+abbrev invariants: Bytes.PartialInvariants SubF := Random.Random.invariants
+
+public
+def Random.invariantsProofs [BytesInvariants]: Bytes.PartialInvariantsProofs Random.invariants where
+  usage_later := by
+    intro x rec tr1 tr2
+    let {timestamp, size} := x
+    simp_all [invariants, DY.ALaCarte.FunctorSizeOf.sizeOf, GetUsageLaterT, Trace.at_le tr1 tr2 timestamp]
+    grind [Trace.at_is_imp_proofProj_at]
+
+  label_later := by
+    intro _ x rec tr1 tr2
+    let {timestamp, size} := x
+    simp_all [invariants, DY.ALaCarte.FunctorSizeOf.sizeOf, GetLabelLaterT, Trace.at_le tr1 tr2 timestamp]
+    grind [Trace.at_is_imp_proofProj_at]
+
+public
+abbrev invariantsProofs [BytesInvariants]: Bytes.PartialInvariantsProofs invariants := Random.Random.invariantsProofs
+
+variable [BytesInvariants] [BytesInvariants.Has invariants]
+
+theorem makeRand.Invariant
+  (timestamp size: Nat) (tr: ProofTrace)
+  (label: Label) (usage: Usage)
+  : Trace.at_is tr timestamp ({ length := size, label := label, usage := usage }: ProofEntryT) → (
+      (makeRand timestamp size: Bytes).Invariant tr ∧
+      (makeRand timestamp size: Bytes).label tr = label ∧
+      (makeRand timestamp size: Bytes).HasUsage usage tr
+    )
+:= by
+  simp [makeRand, Bytes.label.eq, Bytes.usage.eq, Bytes.HasUsage, Bytes.Invariant.eq, Random.invariants]
+  grind [Trace.at_is_imp_proofProj_at]
+
+end Invariants
+
+section AttackerKnowledgeTheorem
+
+variable [TraceInvariant]
+variable [BytesFunctor] [BytesInvariants]
+variable [BytesFunctor.Has SubF]
+variable [TraceTypes.Has ProofEntryFunc]
+variable [BytesInvariants.Has invariants]
+
+public
+instance: SubAttackerKnowledgeTheorem attKnowsRand where
+  pf := by simp [attKnowsRand]
+
+example: SubAttackerKnowledgeTheorem attackerKnowledge := inferInstance
+
+end AttackerKnowledgeTheorem
+
+end Bytes
+
+public
+def genRand [BytesFunctor] [BytesFunctor.Has SubF] [ExecTraceTypes] [ExecTraceTypes.Has ExecEntryT] (size: Nat): Traceful Bytes :=
+  do
+  let entry: ExecEntryT := { length := size }
+  let time ← appendEntry entry
+  return makeRand time size
+
+public
+instance
+  [BytesFunctor] [BytesFunctor.Has SubF] [ExecTraceTypes] [ExecTraceTypes.Has ExecEntryT]
+  (size: Nat)
+  : HasGhostArgumentType (genRand size) (Label × Usage)
+where
+  dummy := ()
+
+@[instance]
+public
+theorem genRand.spec
+  [BytesFunctor]
+  [TraceInvariant]
+  [BytesInvariants] [BytesInvariantsProofs]
+  [BytesFunctor.Has SubF]
+  [TraceInvariant.Has Invariant]
+  [BytesInvariants.Has invariants]
+  (size: Nat)
+  (label: Label) (usage: Usage)
+  : HoareTripleGhost
+    (genRand size)
+    (label, usage)
+    (fun _ => True)
+    (fun res tr =>
+      -- length?
+      -- last event in the trace? (for injectivity properties)
+      res.Invariant tr ∧
+      res.label tr = label ∧
+      res.HasUsage usage tr
+    )
+:= by
+  apply HoareTripleGhost.mk
+  unfold genRand
+  dsimp only
+  step with ⟨ ProofEntryT.mk size label usage ⟩ by
+    simp_all [ProofEntryFunc, Invariant]
+  step
+  grind [makeRand.Invariant]
+
+end DY.Random
